\documentclass[10pt, a4paper]{article}
\usepackage[UTF8]{ctex}
\usepackage[top=3cm, bottom=4cm, left=3.5cm, right=3.5cm]{geometry}
\usepackage{amsmath,amsthm,amsfonts,amssymb,amscd, fancyhdr, color, comment, graphicx, environ} % Mathtools
\usepackage{float}
\usepackage{mathrsfs}
\usepackage[math-style=ISO]{unicode-math}
\setmathfont{Latin Modern Math}
\usepackage{anyfontsize} %字体大小
\usepackage{tikz} %画图

\begin{document}

\section{Randomized Trials} 
\subsection{Causal Effect}
Difference between the treatment group and the control group.
First we can construct a dummy variable $D_i$ to indicate whether the $i$-th component is in the treatment group or the control group:
\[D_i = \begin{cases}
1, & \text{if the $i$-th component is in the treatment group} \\
0, & \text{if the $i$-th component is in the control group}
\end{cases}\]

\[\text{Diffenence in group means} = Avg_n[Y_{1i} \mid D_i = 1] - Avg_n[Y_{0i} \mid D_i = 0] \]
But this equation is not what we are looking for. (Why? Not the comparasion between apples and apples.) We use \kappa to denote the effect of the treatment, then we have:
\[ Y_{1i} = Y_{0i} + \kappa \]
\begin{align*}
    \text{Diffenence in group means} &= Avg_n[Y_{1i} \mid D_i = 1] - Avg_n[Y_{0i} \mid D_i = 0] \\
    &= {\kappa + Avg_n[Y_{0i} \mid D_i = 1]} - Avg_n[Y_{0i} \mid D_i = 0] \\
    &= \kappa + \{Avg_n[Y_{0i} \mid D_i = 1] - Avg_n[Y_{0i} \mid D_i = 0]\}
\end{align*}
According to this, the difference between the two groups can be written as:
\[\boxed{\text{Diffenence in group means} = \text{Average causal effect} + \text{Section bias }}\]  

\subsection{Fundamental Knowledge of Inference}
\begin{itemize}
    \item \textbf{Unbiasedness of the sample mean:} $E[\bar{Y}] = E[Y_i]$
    \item \textbf{Variance of the sample mean:} $Var[\bar{Y}] = \frac{\sigma^2_Y}{n}$
    \item \textbf{the Estimated standard error:} $\hat{SE}(\bar{Y}) = \frac{S(Y_i)}{\sqrt{n}}$
    \item \textbf{the Estimated standard error of the difference in means:} \\
    $\hat{SE}(\bar{Y}_1 - \bar{Y}_0) = \sigma_Y \sqrt{\frac{1}{n_1} + \frac{1}{n_0}}$
    \item \textbf{the t-statistic for the difference in means:} \\
    $t(\mu) = \frac{\bar{Y}_1 - \bar{Y}_0 - \mu}{\hat{SE}(\bar{Y}_1 - \bar{Y}_0)}$
\end{itemize} 

\end{document}